Removed Inside Operation

Rocq/src/Utils.v
@@ -40,25 +40,71 @@ Module Utils.
   Lemma mapI_values :  forall (X Y: Type) (f: nat -> X -> Y) (l: list X) y,
       In y (mapI f l) <-> exists n x, nth_error l n = Some x /\ y = f n x.
   Proof.
-    intros. unfold mapI.  apply mapI'_values.
+    intros. unfold mapI. apply mapI'_values.
   Qed.
 
-  Definition max_list x l := forall e, In e l -> e <= x.
+  Fixpoint maxList x l :=
+    match l with
+    | [] => x
+    | hd :: tl => max hd (maxList x tl)
+    end
+  .
 
-  Lemma max_in_list : forall x l, max_list x l \/ (exists e, In e l /\ max_list e l /\ x <= e).
+  Lemma maxList_order : forall x hd tl, hd <= x -> max hd (maxList x tl) = maxList x tl.
   Proof.
-    unfold max_list. induction l; intros.
-    - left. intros. inv H.
-    - inv IHl.
-      + destruct (le_ge_dec a x).
-        * left. intros. inv H0; firstorder.
-        * right. exists a. split. firstorder. split. intros. inv H0. reflexivity.
-          apply le_trans with (m := x). firstorder. assumption. assumption.
-      + destruct H as [m [H1 [H2 H3]]]. destruct (le_ge_dec a m).
-        * right. exists m. split. firstorder. split. intros. inv H. assumption. firstorder.
-          assumption.
-        * right. exists a. split. firstorder. split. intros. inv H. reflexivity.
-          apply le_trans with (m := m). firstorder. assumption.
-          apply le_trans with (m := m). assumption. assumption.
+    intros. generalize dependent x. generalize dependent hd. induction tl.
+    - apply max_r.
+    - intros. simpl. destruct (le_ge_dec a (maxList x tl)).
+      + rewrite -> (max_r _ _ l). apply (IHtl _ _ H).
+      + rewrite -> (max_l _ _ g). apply max_r. clear IHtl. induction tl.
+        * apply (le_trans _ _ _ H g).
+        * apply IHtl. apply (max_lub_r _ _ _ g).
   Qed.
+
+  Lemma maxList_val : forall x l, maxList x l = x \/ (exists e, In e l /\ maxList x l = e).
+  Proof.
+    induction l.
+    - left. reflexivity.
+    - destruct IHl.
+      + destruct (le_ge_dec a x).
+        * left. simpl. rewrite (maxList_order _ _ _ l0). assumption.
+        * right. exists a. firstorder. simpl. apply max_l. rewrite <- H in g. assumption.
+      + destruct H as [e [H1 H2]]. destruct (le_ge_dec a e).
+        * right. exists e. split. right. assumption. simpl. subst. apply max_r. assumption.
+        * right. exists a. firstorder. simpl. apply max_l. subst. assumption.
+  Qed.
+
+  Lemma maxList_is_max_l : forall x l, x <= maxList x l.
+  Proof.
+    induction l.
+    - constructor.
+    - apply le_trans with (m := maxList x l). assumption. apply le_max_r.
+  Qed.
+
+  Lemma maxList_is_max_r : forall x l e, In e l -> e <= maxList x l.
+  Proof.
+    induction l; intros.
+    - inversion H.
+    - destruct H.
+      + subst. apply le_max_l.
+      + apply le_trans with (m := maxList x l). firstorder. apply le_max_r.
+  Qed.
+
+  Fixpoint sum (l: list nat) :=
+    match l with
+    | [] => 0
+    | hd :: tl => hd + sum tl
+    end
+  .
+
+  Lemma and_with_impl : forall P Q, P -> (P -> Q) -> P /\ Q.
+  Proof.
+    split; intros; auto.
+  Qed.
+
+  Ltac splitAnd :=
+    match goal with
+    | [ |- _ /\ _ ] => apply and_with_impl; [idtac|intros]
+    end
+  .
 End Utils.
