Rocq/src/Spec.v
@@ -1,0 +1,134 @@
+From Stdlib Require Import Lists.List.
+
+From Verilog Require Import Expr.
+From Verilog Require Import Path.
+From Verilog Require Import Utils.
+
+Import ListNotations.
+Import Nat.
+Import Expr.
+Import Path.
+Import Utils.
+
+Set Implicit Arguments.
+
+Module Spec.
+  Section SpecDef.
+    Variable pass1 : Expr -> path -> nat.
+    Variable pass2 : Expr -> path -> nat.
+
+    Definition atom_pass1 :=
+      forall e p op, e @[p] = Some (EAtom op) -> pass1 e p = op.
+
+    Definition binop_pass1 :=
+      forall e p lhs rhs,
+        e @[p] = Some (EBinOp lhs rhs) ->
+        pass1 e p = max (pass1 e (p ++ [Lhs])) (pass1 e (p ++ [Rhs])).
+
+    Definition unop_pass1 :=
+      forall e p arg, e @[p] = Some (EUnOp arg) -> pass1 e p = pass1 e (p ++ [Arg]).
+
+    Definition cast_pass1 :=
+      forall e p arg, e @[p] = Some (ECast arg) -> pass1 e p = pass1 e (p ++ [Arg]).
+
+    Definition comp_pass1 :=
+      forall e p lhs rhs, e @[p] = Some (EComp lhs rhs) -> pass1 e p = 1.
+
+    Definition logic_pass1 :=
+      forall e p lhs rhs, e @[p] = Some (ELogic lhs rhs) -> pass1 e p = 1.
+
+    Definition red_pass1 :=
+      forall e p arg, e @[p] = Some (EReduction arg) -> pass1 e p = 1.
+
+    Definition shift_pass1 :=
+      forall e p lhs rhs, e @[p] = Some (EShift lhs rhs) -> pass1 e p = pass1 e (p ++ [Lhs]).
+
+    Definition assign_pass1 :=
+      forall e p lval arg, e @[p] = Some (EAssign lval arg) -> pass1 e p = lval.
+
+    Definition shiftassign_pass1 :=
+      forall e p lval arg, e @[p] = Some (EShiftAssign lval arg) -> pass1 e p = lval.
+
+    Definition cond_pass1 :=
+      forall e p cond lhs rhs,
+        e @[p] = Some (ECond cond lhs rhs) ->
+        pass1 e p = max (pass1 e (p ++ [Lhs])) (pass1 e (p ++ [Rhs])).
+
+    Definition concat_pass1 :=
+      forall e p args pList,
+        e @[p] = Some (EConcat args) ->
+        (forall i, nth_error pList i = Some (pass1 e (p ++ [Args i]))) ->
+        pass1 e p = sum pList.
+
+    Definition repl_pass1 :=
+      forall e p i arg, e @[p] = Some (ERepl i arg) -> pass1 e p = i * pass1 e (p ++ [Arg]).
+
+
+
+    Definition sd e p := pass2 e p = pass1 e p.
+
+
+
+    Definition binop_pass2 :=
+      forall e p lhs rhs,
+        e @[p] = Some (EBinOp lhs rhs) ->
+        pass2 e (p ++ [Lhs]) = pass2 e p /\ pass2 e (p ++ [Rhs]) = pass2 e p.
+
+    Definition unop_pass2 :=
+      forall e p arg, e @[p] = Some (EUnOp arg) -> pass2 e (p ++ [Arg]) = pass2 e p.
+
+    Definition cast_pass2 :=
+      forall e p arg, e @[p] = Some (ECast arg) -> sd e (p ++ [Arg]).
+
+    Definition comp_pass2 :=
+      forall e p lhs rhs,
+        e @[p] = Some (EComp lhs rhs) ->
+        forall s, s = max (pass1 e (p ++ [Lhs])) (pass1 e (p ++ [Rhs])) ->
+             pass2 e (p ++ [Lhs]) = s /\ pass2 e (p ++ [Rhs]) = s.
+
+    Definition logic_pass2 :=
+      forall e p lhs rhs,
+        e @[p] = Some (ELogic lhs rhs) -> sd e (p ++ [Lhs]) /\ sd e (p ++ [Rhs]).
+
+    Definition red_pass2 :=
+      forall e p arg, e @[p] = Some (EReduction arg) -> sd e (p ++ [Arg]).
+
+    Definition shift_pass2 :=
+      forall e p lhs rhs, e @[p] = Some (EShift lhs rhs) ->
+                     sd e (p ++ [Rhs]) /\ pass2 e (p ++ [Lhs]) = pass2 e p.
+
+    Definition assign_pass2 :=
+      forall e p lval arg,
+        e @[p] = Some (EAssign lval arg) ->
+        forall s, s = max (pass1 e (p ++ [Arg])) lval -> pass2 e (p ++ [Arg]) = s.
+
+    Definition shiftassign_pass2 :=
+      forall e p lval arg, e @[p] = Some (EShiftAssign lval arg) -> sd e (p ++ [Arg]).
+
+    Definition cond_pass2 :=
+      forall e p cond lhs rhs,
+        e @[p] = Some (ECond cond lhs rhs) ->
+        pass2 e (p ++ [Lhs]) = pass2 e p /\ pass2 e (p ++ [Rhs]) = pass2 e p /\
+          sd e (p ++ [Cond]).
+
+    Definition concat_pass2 :=
+      forall e p args, e @[p] = Some (EConcat args) ->
+                  forall i, i < length args -> sd e (p ++ [Args i]).
+
+    Definition repl_pass2 :=
+      forall e p i arg, e @[p] = Some (ERepl i arg) -> sd e (p ++ [Arg]).
+
+    Definition pass1_def :=
+      atom_pass1 /\ binop_pass1 /\ unop_pass1 /\ cast_pass1 /\
+        comp_pass1 /\ logic_pass1 /\ red_pass1 /\ shift_pass1 /\
+        assign_pass1 /\ shiftassign_pass1 /\ cond_pass1 /\ concat_pass1 /\
+        repl_pass1.
+
+    Definition pass2_def :=
+      binop_pass2 /\ unop_pass2 /\ cast_pass2 /\ comp_pass2 /\
+        logic_pass2 /\ red_pass2 /\ shift_pass2 /\ assign_pass2 /\
+        shiftassign_pass2 /\ cond_pass2 /\ concat_pass2 /\ repl_pass2.
+
+    Definition pass_def := pass1_def /\ pass2_def.
+  End SpecDef.
+End Spec.
